first pass at STLC cleaning

Cslib/Languages/LambdaCalculus/LocallyNameless/Stlc/StrongNorm.lean
@@ -31,7 +31,6 @@ variable {Var : Type u} {Base : Type v} [DecidableEq Var] [HasFresh Var]
 open LambdaCalculus.LocallyNameless.Stlc
 open scoped Term
 
-
 /-- A set of terms is called saturated if it
 
     1. only contains locally closed terms,
@@ -39,14 +38,12 @@ open scoped Term
     3. contains all neutral locally closed terms, and
     4. is closed under top-level β-reduction of the form (λ M) N P₁ … Pₙ → M ^ N P₁ … Pₙ.
 -/
-abbrev saturated (S : Set (Term Var)) : Prop :=
-          (∀ M ∈ S, LC M) ∧
-          (∀ M ∈ S, SN M) ∧
-          (∀ M, Neutral M → LC M → M ∈ S) ∧
-          (∀ M N P, LC N →
-                    SN N →
-                    multiApp (M ^ N) P ∈ S →
-                      multiApp ((Term.abs M).app N) P ∈ S)
+@[scoped grind]
+structure Saturated (S : Set (Term Var)) : Prop where
+  lc : ∀ M ∈ S, LC M
+  sn : ∀ M ∈ S, SN M
+  neutal_lc : ∀ M, Neutral M → LC M → M ∈ S
+  multiApp : ∀ M N P, LC N → SN N → multiApp (M ^ N) P ∈ S → multiApp (M.abs.app N) P ∈ S
 
 /-- The semantic map maps each type to a corresponding saturated set of terms.
     For the strong normalization proof to work, we must ensure that
@@ -55,71 +52,44 @@ abbrev saturated (S : Set (Term Var)) : Prop :=
     Strong normalization later follows from the fact that terms in saturated
     sets are strongly normalizing.
 -/
-@[simp, grind]
-def semanticMap (τ : Ty Base) : Set (Term Var) :=
-  match τ with
-  | Ty.base _ => { t : Term Var | SN t ∧ LC t }
-  | Ty.arrow τ₁ τ₂ =>
-    { t : Term Var | ∀ s : Term Var, s ∈ semanticMap τ₁ → (Term.app t s) ∈ semanticMap τ₂ }
-
+@[simp, scoped grind =]
+def semanticMap : Ty Base → Set (Term Var)
+  | .base _ => { t | SN t ∧ LC t }
+  | .arrow τ₁ τ₂ => { t | ∀ s, s ∈ semanticMap τ₁ → app t s ∈ semanticMap τ₂ }
 
 /-- The sets constructed by semanticMap are saturated -/
-lemma semanticMap_saturated (τ : Ty Base) :
-    @saturated Var (semanticMap τ) := by
-  induction τ
-  · case base b => grind[sn_abs_app_multiApp, sn_neutral, multiApp_lc, open_abs_lc]
-  · case arrow τ₁ τ₂ ih₁ ih₂ =>
-      constructor
-      · intro M hM
-        have H := ih₁.2.2.1 (.fvar (fresh {})) (.fvar (fresh {})) (.fvar (fresh {}))
-        specialize (hM (fvar (fresh {})) H)
-        apply (ih₂.1) at hM
-        cases hM
-        assumption
-      · constructor
-        · intro M hM
-          apply sn_app_left M (Term.fvar (fresh {})) <;> grind
-        · constructor
-          · grind
-          · intro M N P lc_N sn_N h_app s hs
-            apply ih₂.2.2.2 M N (s::P) <;> grind
-
-
-
+lemma semanticMap_saturated (τ : Ty Base) : @Saturated Var (semanticMap τ) := by
+  induction τ with
+  | base => grind [sn_abs_app_multiApp, sn_neutral, open_abs_lc]
+  | arrow τ₁ τ₂ ih₁ ih₂ =>
+    constructor
+    · grind [ih₁.neutal_lc (fvar <| fresh {}) (.fvar <| fresh {}) (.fvar <| fresh {}), cases LC]
+    · grind [sn_app_left (Var := Var) (N := fvar <| fresh {})]
+    · grind
+    · intro M N P _ _ _ s _
+      grind [ih₂.multiApp M N (s :: P)]
 
 /-- The `entails_context` predicate ensures that each variable in the context
     is mapped to a term in the corresponding semantic map. -/
 abbrev entails_context (E : Term.Env Var) (Γ : Context Var (Ty Base)) :=
-  ∀ {x τ}, ⟨ x, τ ⟩ ∈ Γ → (multiSubst E (Term.fvar x)) ∈ semanticMap τ
+  ∀ {x τ}, ⟨x, τ⟩ ∈ Γ → (multiSubst E (fvar x)) ∈ semanticMap τ
 
 /-- The empty context is entailed by any environment. -/
-lemma entails_context_empty {Γ : Context Var (Ty Base)} :
-  entails_context [] Γ := by
-  intro x τ h_mem
-  have Hsat := (@semanticMap_saturated Var Base _ _ τ)
+lemma entails_context_empty {Γ : Context Var (Ty Base)} : entails_context [] Γ := by
+  have := semanticMap_saturated (Var := Var) (Base := Base)
   grind
 
+open scoped Context in
 omit [HasFresh Var] in
 /-- The `entails_context` predicate is preserved when extending the context
     with a new variable, provided the new variable is fresh and its
     substitution is in the corresponding semantic map. -/
 lemma entails_context_cons (E : Term.Env Var) (Γ : Context Var (Ty Base))
-  (x : Var) (τ : Ty Base) (sub : Term Var)
-  (h_fresh : x ∉ E.dom ∪ E.fv ∪ Γ.dom)
-  (h_mem : sub ∈ semanticMap τ) :
+    (x : Var) (τ : Ty Base) (sub : Term Var)
+    (h_fresh : x ∉ E.dom ∪ E.fv ∪ Γ.dom)
+    (h_mem : sub ∈ semanticMap τ) :
     entails_context E Γ → entails_context (⟨ x, sub ⟩ :: E) (⟨ x, τ ⟩ :: Γ) := by
-  intro h_entails y σ h_mem
-  rw[multiSubst]
-  rw[entails_context] at h_entails
-  cases h_mem
-  · case head       => grind [multiSubst_fvar_fresh]
-  · case tail h_mem =>
-    specialize (h_entails h_mem)
-    rw [subst_fresh]
-    · assumption
-    · apply multiSubst_preserves_not_fvar
-      apply List.mem_keys_of_mem at h_mem
-      aesop
+  grind [multiSubst_fvar_fresh, subst_fresh, multiSubst_preserves_not_fvar]
 
 /-- The `entails` predicate states that a term `t` is
     semantically valid with respect to a context `Γ` and a type `τ` -/
@@ -128,26 +98,25 @@ abbrev entails (Γ : Context Var (Ty Base)) (t : Term Var) (τ : Ty Base) :=
 
 /-- The `soundness` lemma states that if a term `t` has type `τ` in context `Γ`,
     then `t` is semantically valid with respect to `Γ` and `τ` -/
-lemma soundness {Γ : Context Var (Ty Base)} {t : Term Var} {τ : Ty Base}
-    (derivation_t : Γ ⊢ t ∶ τ) : entails Γ t τ := by
-  induction derivation_t
-  · case var Γ xσ_mem_Γ => grind
-  · case' abs σ Γ t τ L HL IH =>
-      have sat_semMap_τ := (@semanticMap_saturated Var Base _ _ τ)
-      have sat_semMap_σ := (@semanticMap_saturated Var Base _ _ σ)
-      intro E lc_E hsat s hsat_s
-      have ⟨x, Hfresh⟩ :=
-        fresh_exists <| (t.fv ∪ L ∪ E.dom ∪ E.fv ∪ Context.dom Γ ∪ (multiSubst E t).fv)
-      specialize IH x (by simp_all) (⟨x,s⟩ :: E)
-      rw[multiSubst_abs]
-      apply sat_semMap_τ.2.2.2 _ _ [] <;> grind[entails_context_cons, multiSubst_open_var]
-  · case app derivation_t derivation_t' IH IH' => grind[multiSubst_app]
+lemma soundness {Γ : Context Var (Ty Base)} (derivation_t : Γ ⊢ t ∶ τ) : entails Γ t τ := by
+  induction derivation_t with
+  | var Γ xσ_mem_Γ => grind
+  | @abs σ Γ t τ L HL IH =>
+    intro E _ _ s
+    have sat_semMap_σ := semanticMap_saturated (Var := Var) σ
+    have sat_semMap_τ := semanticMap_saturated (Var := Var) τ
+    have := sat_semMap_τ.multiApp (multiSubst E t) s []
+    let := multiSubst E t
+    have ⟨x, _⟩ := fresh_exists <| E.dom ∪ free_union [fv, Context.dom, Env.fv] Var
+    have := IH (x := x) (E := ⟨x,s⟩ :: E)
+    grind [multiSubst_abs, entails_context_cons, multiSubst_open_var]
+  | app => grind [multiSubst_app]
 
 /-- Using soundness and the fact that the empty context
     is entailed by any environment, we can conclude that
     a well-typed term is strongly normalizing. -/
 theorem strong_norm {t : Term Var} {τ : Ty Base} (der : Γ ⊢ t ∶ τ) : SN t := by
-  apply (semanticMap_saturated τ).2.1
+  apply (semanticMap_saturated τ).sn
   apply (soundness der [] (by grind) entails_context_empty)
 
 end LambdaCalculus.LocallyNameless.Stlc
